CpcMini/Proofs/TypePreservation/Support.lean
@@ -74,9 +74,9 @@ inductive supported_preservation_term : SmtTerm -> Prop
       supported_preservation_term (SmtTerm.imp t1 t2)
   | eq (t1 t2 : SmtTerm) :
       supported_preservation_term (SmtTerm.eq t1 t2)
-  | dt_cons (s : native_String) (d : SmtDatatype) (i : native_Nat) :
+  | dt_cons (s : native_String) (d : SmtDatatypeDecl) (i : native_Nat) :
       supported_preservation_term (SmtTerm.DtCons s d i)
-  | dt_sel {s : native_String} {d : SmtDatatype} {i j : native_Nat} {x : SmtTerm}
+  | dt_sel {s : native_String} {d : SmtDatatypeDecl} {i j : native_Nat} {x : SmtTerm}
       (ht : term_has_non_none_type (SmtTerm.Apply (SmtTerm.DtSel s d i j) x))
       (hT : type_inhabited (__smtx_typeof (SmtTerm.Apply (SmtTerm.DtSel s d i j) x)))
       (hWrongMapWF :
@@ -87,7 +87,7 @@ inductive supported_preservation_term : SmtTerm -> Prop
       (htx : term_has_non_none_type x)
       (hsx : supported_preservation_term x) :
       supported_preservation_term (SmtTerm.Apply (SmtTerm.DtSel s d i j) x)
-  | dt_tester (s : native_String) (d : SmtDatatype) (i : native_Nat) (x : SmtTerm) :
+  | dt_tester (s : native_String) (d : SmtDatatypeDecl) (i : native_Nat) (x : SmtTerm) :
       supported_preservation_term (SmtTerm.Apply (SmtTerm.DtTester s d i) x)
   | apply {f x : SmtTerm}
       (hTy : generic_apply_type f x)
